OO mem is fixed

Phi_Semantics/PhiSem_OO_Class_Algebra.thy
@@ -1,5 +1,5 @@
 theory PhiSem_OO_Class_Algebra
-  imports Phi_System.PhiSem_Formalization_Tools
+  imports PhiSem_Base
 begin
 
 section \<open>Algebraic Model of Class dependency\<close>
@@ -96,6 +96,14 @@ definition inherited_members_of :: \<open>'m class_algebra \<Rightarrow> 'm::com
   where \<open>inherited_members_of cls = prod class_algebra.members (self_and_parents_of cls)\<close>
 
 
+type_synonym "class" = \<open>(field_name \<rightharpoonup> TY nosep) class_algebra\<close>
+
+setup \<open>Sign.mandatory_path "class"\<close>
+
+abbreviation fields_of :: \<open>class \<Rightarrow> field_name \<rightharpoonup> TY nosep\<close>
+  where \<open>fields_of \<equiv> inherited_members_of\<close>
+
+setup \<open>Sign.parent_path\<close>
 
 
 end
