Phi_Semantics/PhiSem_Mem_C.thy
@@ -1,0 +1,860 @@
+theory PhiSem_Mem_C
+  imports PhiSem_Mem_C_Base "HOL-Library.Word"
+begin
+
+section \<open>Semantics\<close>
+
+subsection \<open>Models\<close>
+
+subsubsection \<open>Type\<close>
+
+virtual_datatype c_mem_ty =
+  T_pointer :: unit
+
+debt_axiomatization T_pointer :: \<open>unit type_entry\<close>
+  where c_mem_ty_ax: \<open>c_mem_ty TY_CONS_OF T_pointer\<close>
+
+interpretation c_mem_ty TY_CONS_OF \<open>TYPE(TY_N)\<close> \<open>TYPE(TY)\<close> T_pointer using c_mem_ty_ax .
+
+abbreviation \<open>pointer \<equiv> T_pointer.mk ()\<close>
+
+
+subsubsection \<open>Value\<close>
+
+paragraph \<open>Memory Address\<close>
+
+consts addrspace_bits :: "nat" \<comment> \<open>bit width of address space, in unit of bits\<close>
+specification (addrspace_bits) addrspace_bits_L0: "0 < addrspace_bits" by blast
+
+typedecl addr_cap \<comment> \<open>size of address space\<close>
+
+instantiation addr_cap :: len begin
+definition [simp]: "len_of_addr_cap (_::addr_cap itself) = addrspace_bits"
+instance apply standard using addrspace_bits_L0 by simp
+end
+
+type_synonym size_t = \<open>addr_cap word\<close>
+abbreviation to_size_t :: \<open>nat \<Rightarrow> size_t\<close> where \<open>to_size_t \<equiv> of_nat\<close>
+
+declare [[typedef_overloaded]]
+datatype segidx = Null | Segment nat \<comment> \<open>nonce\<close> (layout: TY)
+
+hide_const (open) layout
+
+datatype 'index memaddr = memaddr (segment: segidx) (index: 'index) (infixl "|:" 60)
+declare [[typedef_overloaded = false]]
+
+declare memaddr.sel[iff]
+hide_const (open) segment index
+
+type_synonym logaddr = "nat list memaddr" (* the index of logaddr is non empty *)
+type_synonym rawaddr = \<open>size_t memaddr\<close> \<comment> \<open>having physical offset\<close>
+
+instantiation segidx :: zero begin
+definition [simp]: "zero_segidx = Null"
+instance ..
+end
+
+instantiation memaddr :: (zero) zero begin
+definition "zero_memaddr = (0 |: 0)"
+instance ..
+end
+
+
+lemma infinite_UNIV_int [simp]: "infinite (UNIV::int set)"
+proof
+  assume "finite (UNIV::int set)"
+  moreover have "inj (\<lambda>i::int. 2 * i)"
+    by (rule injI) simp
+  ultimately have "surj (\<lambda>i::int. 2 * i)"
+    by (rule finite_UNIV_inj_surj)
+  thm finite_UNIV_inj_surj
+  then obtain i :: int where "1 = 2 * i" by (rule surjE)
+  then show False by presburger
+qed
+
+lemma segidx_infinite[simp]:
+  \<open>infinite (UNIV :: segidx set)\<close>
+  using inj_on_finite[where A = \<open>UNIV::nat set\<close> and B = \<open>(UNIV :: segidx set)\<close>
+        and f = \<open>\<lambda>n. Segment n undefined\<close>]
+  by (meson infinite_UNIV_char_0 injI segidx.inject top_greatest)
+
+lemma segidx_infinite_TY:
+  \<open>infinite {a. segidx.layout a = TY}\<close>
+  using inj_on_finite[where A = \<open>UNIV::nat set\<close> and B = \<open>{a. segidx.layout a = TY}\<close>
+        and f = \<open>\<lambda>n. Segment n TY\<close>]
+  using inj_def by fastforce
+
+
+abbreviation shift_addr :: "'idx memaddr \<Rightarrow> ('idx::monoid_add) \<Rightarrow> 'idx memaddr" (infixl "||+" 60)
+  where "shift_addr addr delta \<equiv> map_memaddr (\<lambda>x. x + delta) addr"
+
+lemma mem_shift_shift[simp]: "a ||+ i ||+ j = a ||+ (i + j)" by (cases a) (simp add: add.assoc)
+
+lemma memaddr_segment_shift[simp]:
+  \<open>memaddr.segment (a ||+ i) = memaddr.segment a\<close>
+  by (cases a, simp)
+
+lemma memaddr_index_shift[simp]:
+  \<open>memaddr.index (a ||+ i) = memaddr.index a + i\<close>
+  by (cases a, simp)
+
+lemma mem_shift_add_cancel[simp]:
+  \<open>(a ||+ i) = (a ||+ j) \<longleftrightarrow> i = j\<close>
+  for i :: \<open>'a::{monoid_add,cancel_semigroup_add}\<close>
+  by (cases a, simp)
+
+
+
+paragraph \<open>Model\<close>
+
+virtual_datatype c_mem_val = V_pointer :: rawaddr
+
+debt_axiomatization V_pointer :: \<open>rawaddr value_entry\<close>
+  where c_mem_val_ax: \<open>c_mem_val VAL_CONS_OF V_pointer\<close>
+
+interpretation c_mem_val VAL_CONS_OF \<open>TYPE(VAL_N)\<close> \<open>TYPE(VAL)\<close> V_pointer using c_mem_val_ax .
+
+
+subsubsection \<open>Resource\<close>
+
+setup \<open>Sign.mandatory_path "RES"\<close>
+
+type_synonym mem = \<open>segidx \<rightharpoonup> VAL nosep\<close>
+
+setup \<open>Sign.parent_path\<close>
+
+resource_space c_mem =
+  mem :: \<open>{h::RES.mem. finite (dom h) \<and> (\<forall>seg \<in> dom h. h seg \<in> Some ` nosep ` Well_Type (segidx.layout seg))}\<close>
+  .
+
+definition In_Mem :: \<open> resource \<Rightarrow> segidx \<Rightarrow> bool\<close>
+  where \<open>In_Mem res seg \<equiv> seg \<in> dom (RES.mem.get res)\<close>
+
+
+subsection \<open>Semantics\<close>
+
+abbreviation \<open>type_storable_in_mem T \<equiv> MemObj_Size T < 2^addrspace_bits\<close>
+
+definition \<open>Valid_Segment seg = (
+    case seg of Null \<Rightarrow> True
+              | Segment _ ty \<Rightarrow> type_storable_in_mem ty
+    )\<close>
+
+lemma Valid_Segment_zero[simp]: \<open>Valid_Segment Null\<close>
+  unfolding Valid_Segment_def zero_segidx_def by simp
+
+abbreviation valid_rawaddr :: \<open>rawaddr \<Rightarrow> bool\<close>
+  where \<open>valid_rawaddr addr \<equiv> Valid_Segment (memaddr.segment addr)\<close>
+
+definition valid_logaddr :: "logaddr \<Rightarrow> bool"
+  where "valid_logaddr addr \<longleftrightarrow>
+    Valid_Segment (memaddr.segment addr) \<and>
+    (memaddr.segment addr = Null \<longrightarrow> memaddr.index addr = []) \<and>
+    valid_index (segidx.layout (memaddr.segment addr)) (memaddr.index addr)"
+
+lemma valid_rawaddr_0[simp]: \<open>valid_rawaddr (0 |: 0)\<close>
+  by (simp add: zero_prod_def Valid_Segment_def zero_memaddr_def zero_segidx_def)
+
+lemma valid_logaddr_0[simp]: \<open>valid_logaddr (0 |: [])\<close>
+  by (simp add: valid_logaddr_def zero_prod_def Valid_Segment_def zero_memaddr_def zero_segidx_def)
+
+
+
+debt_axiomatization
+    can_eqcmp_ptr[simp]: "Can_EqCompare res (V_pointer.mk rp1) (V_pointer.mk rp2)
+           \<longleftrightarrow> (memaddr.segment rp1 = memaddr.segment rp2) \<or> (rp1 = 0) \<or> (rp2 = 0) \<or>
+               (In_Mem res (memaddr.segment rp1) \<and> In_Mem res (memaddr.segment rp2))"
+and eqcmp_ptr[simp]: "EqCompare (V_pointer.mk rp1) (V_pointer.mk rp2) \<longleftrightarrow> rp1 = rp2"
+and zero_ptr[simp]: \<open>Zero pointer = Some (V_pointer.mk 0)\<close>
+and WT_ptr[simp]: \<open>Well_Type \<tau>Pointer = { V_pointer.mk addr |addr. valid_rawaddr addr }\<close>
+
+
+(*
+definition Valid_Mem :: "('TY,'VAL) R_mem set"
+  where "Valid_Mem = { Fine h |h. finite (dom h)
+                                \<and> (\<forall>seg \<in> dom h. h seg \<in> Some ` Well_Type (segidx.layout seg))}"
+
+lemma Valid_Mem_1[simp]: \<open>1 \<in> Valid_Mem\<close>
+  unfolding Valid_Mem_def one_fun_def one_fine_def by simp
+*)
+
+lemma Mem_freshness:
+  \<open>finite (dom f) \<Longrightarrow> \<exists>k. f k = None \<and> segidx.layout k = TY\<close>
+  unfolding dom_def
+  by (smt (verit, del_insts) Collect_mono finite_Collect_disjI finite_subset segidx_infinite_TY)
+
+
+paragraph \<open>Address & Pointer\<close>
+
+abbreviation logaddr_type :: \<open>logaddr \<Rightarrow> TY\<close>
+  where \<open>logaddr_type addr \<equiv> index_type (memaddr.index addr) (segidx.layout (memaddr.segment addr))\<close>
+
+lemma MemObj_Size_LE_idx:
+  \<open>valid_index T (base@idx) \<Longrightarrow> MemObj_Size (index_type (base@idx) T) \<le> MemObj_Size (index_type base T)\<close>
+  apply (induct base arbitrary: T idx; simp)
+  subgoal for T idx apply (induct idx arbitrary: T; simp)
+    using memobj_size_step order.trans by blast .
+
+lemmas MemObj_Size_LE_idx_0 = MemObj_Size_LE_idx[where base = "[]", simplified]
+
+lemma index_type_type_storable_in_mem:
+  \<open>type_storable_in_mem T \<Longrightarrow> valid_index T idx \<Longrightarrow> type_storable_in_mem (index_type idx T)\<close>
+  using MemObj_Size_LE_idx_0 order.strict_trans1 by blast 
+
+lemma logaddr_storable_in_mem:
+  \<open>valid_logaddr addr \<Longrightarrow> addr \<noteq> 0 \<Longrightarrow> type_storable_in_mem (logaddr_type addr)\<close>
+  unfolding valid_logaddr_def Valid_Segment_def zero_memaddr_def
+  apply (cases addr; simp)
+  subgoal for seg idx by (cases seg; simp add: index_type_type_storable_in_mem) .
+
+definition logaddr_to_raw :: \<open>logaddr \<Rightarrow> rawaddr\<close>
+  where \<open>logaddr_to_raw addr =
+    (case addr of seg |: idx \<Rightarrow> seg |: to_size_t (index_offset (segidx.layout seg) idx))\<close>
+
+lemma logaddr_to_raw_0[simp]:
+  \<open>logaddr_to_raw (0 |: []) = (0 |: 0)\<close>
+  unfolding logaddr_to_raw_def by simp
+
+lemma logaddr_to_raw_segment[simp]:
+  \<open>memaddr.segment (logaddr_to_raw addr) = memaddr.segment addr\<close>
+  unfolding logaddr_to_raw_def by (cases addr) simp
+
+lemma valid_logaddr_rawaddr [simp]:
+  \<open>valid_logaddr addr \<Longrightarrow> valid_rawaddr (logaddr_to_raw addr)\<close>
+  unfolding valid_logaddr_def by simp 
+
+
+lemma index_offset_inj:
+  assumes prems:
+    \<open>valid_index T index1\<close>
+    \<open>valid_index T index2\<close>
+    \<open>index_type index2 T = index_type index1 T\<close>
+    \<open>0 < MemObj_Size (index_type index1 T)\<close>
+  shows \<open>index_offset T index1 = index_offset T index2 \<longrightarrow> index1 = index2\<close>
+proof -
+  consider (either_nil) \<open>index1 = [] \<or> index2 = []\<close>
+      |   (both_notnil) \<open>index1 \<noteq> [] \<and> index2 \<noteq> []\<close>
+      by blast
+  then show ?thesis
+  proof cases
+    case either_nil
+      then show ?thesis using prems index_type_idem by metis
+  next
+    case both_notnil
+    have \<open>index1 \<noteq> index2 \<longrightarrow> index_offset T index1 \<noteq> index_offset T index2\<close> (is \<open>?neq \<longrightarrow> ?goal\<close>)
+    proof
+      assume neq: ?neq
+
+      have t1: \<open>\<And>idx1 idx2. idx1 \<noteq> [] \<and> idx2 \<noteq> [] \<and> idx1 \<noteq> idx2 \<and> \<not>(\<exists>d. idx1@d = idx2) \<and> \<not>(\<exists>d. idx2@d = idx1)
+          \<Longrightarrow> \<exists>i. i < length idx1 \<and> i < length idx2 \<and> idx1 ! i \<noteq> idx2 ! i \<close>
+        unfolding list_eq_iff_nth_eq nth_append apply simp apply clarify
+        subgoal premises prems for idx1 idx2
+          apply (cases \<open>length idx1 \<le> length idx2\<close>)
+          using prems(4)[THEN spec[where x=\<open>drop (length idx1) idx2\<close>], simplified]
+           apply (metis le_add_diff_inverse linordered_semidom_class.add_diff_inverse nth_drop)
+          using prems(5)[THEN spec[where x=\<open>drop (length idx2) idx1\<close>], simplified]
+           by (metis add_diff_inverse_nat le_add_diff_inverse nat_le_linear nth_drop)
+         done
+
+       moreover have t2: \<open>\<And>i idx1 idx2. i < length idx1 \<and> i < length idx2 \<and> idx1 ! i \<noteq> idx2 ! i
+          \<Longrightarrow> \<exists>i. i < length idx1 \<and> i < length idx2 \<and> idx1 ! i \<noteq> idx2 ! i \<and> take i idx1 = take i idx2\<close>
+         unfolding list_eq_iff_nth_eq apply simp
+         subgoal for i idx1 idx2
+           apply (induct i arbitrary: idx1 idx2 rule: nat_less_induct)
+           by (smt (verit, ccfv_threshold) min.absorb4 min_less_iff_conj)
+         done
+
+       ultimately have t3:
+          \<open>\<And>idx1 idx2. idx1 \<noteq> [] \<and> idx2 \<noteq> [] \<and> idx1 \<noteq> idx2 \<and> \<not>(\<exists>d. idx1@d = idx2) \<and> \<not>(\<exists>d. idx2@d = idx1)
+          \<Longrightarrow> \<exists>i. i < length idx1 \<and> i < length idx2 \<and> idx1 ! i \<noteq> idx2 ! i \<and> take i idx1 = take i idx2\<close>
+         by (smt (verit, ccfv_threshold))
+
+       note t4 = t3[of \<open>index1\<close> \<open>index2\<close>, simplified both_notnil, simplified]
+         
+
+       have \<open>\<not>((\<exists>d. index1@d = index2) \<or> (\<exists>d. index2@d = index1))\<close>
+       proof
+         assume A: \<open>(\<exists>d. index1 @ d = index2) \<or> (\<exists>d. index2 @ d = index1)\<close>
+         then consider (L) \<open>\<exists>d. index1 @ d = index2\<close> |
+                       (R) \<open>(\<exists>d. index2 @ d = index1)\<close> by blast
+         then show False
+         proof cases
+           case L
+           then obtain d where D: \<open>index2 = index1@d\<close> by blast
+           then have \<open>valid_index (index_type index1 T) d\<close> using valid_index_cat prems by blast
+           then have \<open>d = []\<close> using fold_append prems D by (simp add: index_type_idem)
+           then show False using neq D by blast
+         next
+           case R
+           then obtain d where D: \<open>index1 = index2@d\<close> by blast
+           then have \<open>valid_index (index_type index2 T) d\<close> using valid_index_cat prems by blast
+           then have \<open>d = []\<close> using fold_append prems D by (metis comp_def index_type_idem) 
+           then show False using neq D by blast
+         qed
+       qed
+      then have \<open>\<exists>base i1 idx1 i2 idx2. index1 = (base@[i1])@idx1 \<and> index2 = (base@[i2])@idx2 \<and> i1 \<noteq> i2\<close>
+        using neq both_notnil t4
+        by (metis append.assoc append_Cons append_Nil id_take_nth_drop)
+      then obtain base i1 idx1 i2 idx2 where
+        obt: \<open>(base@[i1])@idx1 = index1 \<and> (base@[i2])@idx2 = index2 \<and> i1 \<noteq> i2\<close>
+        by blast
+
+      have valid_idx_step_i1: \<open>valid_idx_step (index_type base T) i1\<close>
+        using prems valid_index_cat valid_index_cons obt by blast
+      have valid_idx_step_i2: \<open>valid_idx_step (index_type base T) i2\<close>
+        using prems valid_index_cat valid_index_cons obt by blast
+      have \<open>index_offset T index1 \<noteq> index_offset T index2\<close>
+        using index_offset_bound_strict[where base = \<open>base@[i1]\<close> and idx = idx1 and T = T,
+                                        simplified index_offset_tail obt prems fold_tail]
+              index_offset_bound_strict[where base = \<open>base@[i2]\<close> and idx = idx2 and T = T,
+                                        simplified index_offset_tail obt prems fold_tail]
+              idx_step_offset_disj[where T = \<open>index_type base T\<close> and i = i1 and j = i2]
+        by (smt (verit, ccfv_SIG) comp_def group_cancel.add1 idx_step_offset_disj nat_add_left_cancel_less nat_le_linear obt order.strict_trans1 valid_idx_step_i1 valid_idx_step_i2)
+      then show ?goal
+        using obt prems by presburger
+    qed
+    then show ?thesis using prems by blast
+    qed
+  qed
+
+lemma logaddr_to_raw_inj:
+    \<open>valid_logaddr addr1 \<Longrightarrow>
+     valid_logaddr addr2 \<Longrightarrow>
+     logaddr_type addr1 = logaddr_type addr2 \<Longrightarrow>
+     0 < MemObj_Size (logaddr_type addr1) \<Longrightarrow>
+     logaddr_to_raw addr1 = logaddr_to_raw addr2 \<longrightarrow> addr1 = addr2\<close>
+  unfolding logaddr_to_raw_def valid_logaddr_def
+  apply (cases addr1; cases addr2; simp)
+  by (smt (verit, ccfv_SIG) Valid_Segment_def add_leD1 index_offset_inj index_offset_upper_bound_0 len_of_addr_cap_def order_le_less_trans segidx.case_eq_if take_bit_nat_eq_self_iff word_of_nat_eq_iff)
+
+definition \<open>rawaddr_to_log T raddr = (@laddr. logaddr_to_raw laddr = raddr \<and> logaddr_type laddr = T \<and> valid_logaddr laddr)\<close>
+
+lemma rawaddr_to_log[simp]:
+  \<open>valid_logaddr addr \<Longrightarrow> 0 < MemObj_Size (logaddr_type addr)
+    \<Longrightarrow> rawaddr_to_log (logaddr_type addr) (logaddr_to_raw addr) = addr\<close>
+  unfolding rawaddr_to_log_def
+  by (rule some_equality, simp) (metis logaddr_to_raw_inj) 
+
+
+
+subsection \<open>Fiction\<close>
+
+definition sem_read_mem :: \<open>logaddr \<Rightarrow> resource \<Rightarrow> VAL\<close>
+  where \<open>sem_read_mem addr res =
+    index_value (memaddr.index addr) (nosep.dest (the (RES.mem.get res (memaddr.segment addr))))\<close>
+
+definition sem_write_mem :: \<open>logaddr \<Rightarrow> VAL \<Rightarrow> resource \<Rightarrow> resource\<close>
+  where \<open>sem_write_mem addr val res =
+    (let seg = memaddr.segment addr
+       ; mem = RES.mem.get res
+       ; val' = index_mod_value (memaddr.index addr) (\<lambda>_. val) (nosep.dest (the (mem seg)))
+       ; mem' = mem(seg \<mapsto> nosep val')
+      in res(RES.mem #= mem'))\<close>
+
+
+
+(*
+
+fiction_space (in agmem_sem) agmem_fic :: \<open>'RES_N \<Rightarrow> 'RES\<close> = \<phi>min_fic +
+  FIC_mem :: share_mem
+
+(* TODO: agmem_sem should be a locale expression! ! *)
+
+
+locale agmem = agmem_fic
+  where TYPES = \<open>TYPE(('TY_N \<Rightarrow> 'TY)
+                    \<times> ('VAL_N \<Rightarrow> 'VAL::nonsepable_semigroup)
+                    \<times> ('RES_N \<Rightarrow> 'RES::{comm_monoid_mult,no_inverse}))\<close>
+    and TYPE'NAME = \<open>TYPE('FIC_N)\<close>
+    and TYPE'REP = \<open>TYPE('FIC::{no_inverse,comm_monoid_mult})\<close> 
++ fixes TYPES :: \<open>(('TY_N \<Rightarrow> 'TY) \<times> ('VAL_N \<Rightarrow> 'VAL) \<times> ('RES_N \<Rightarrow> 'RES) \<times> ('FIC_N \<Rightarrow> 'FIC)) itself\<close>
+begin
+
+lemma R_mem_valid_split: \<open>res \<in> Valid_Resource \<longleftrightarrow>
+    R_mem.clean res \<in> Valid_Resource \<and> (\<exists>m. res R_mem.name = R_mem.inject m \<and> m \<in> Valid_Mem)\<close>
+  by (subst R_mem.split, simp add: Valid_Resource_def times_fun_def res_valid_mem image_iff, blast)
+     
+
+lemma R_mem_valid_split': \<open>NO_MATCH (R_mem.clean res') res \<Longrightarrow> res \<in> Valid_Resource \<longleftrightarrow>
+    R_mem.clean res \<in> Valid_Resource \<and> (\<exists>m. res R_mem.name = R_mem.inject m \<and> m \<in> Valid_Mem)\<close>
+  using R_mem_valid_split .
+
+end
+*)
+
+section \<open>\<phi>Type for Semantic Models\<close>
+
+subsection \<open>Pointers\<close>
+
+subsubsection \<open>Raw Pointer\<close>
+
+definition RawPointer :: "(VAL, rawaddr) \<phi>"
+  where "RawPointer x = ({ V_pointer.mk x } \<s>\<u>\<b>\<j> valid_rawaddr x)"
+
+lemma RawPointer_expn[\<phi>expns]:
+  "v \<in> (p \<Ztypecolon> RawPointer) \<longleftrightarrow> v = V_pointer.mk p \<and> valid_rawaddr p"
+  by (simp add: \<phi>Type_def RawPointer_def \<phi>expns)
+
+lemma RawPointer_inhabited[elim!, \<phi>inhabitance_rule]:
+  "Inhabited (p \<Ztypecolon> RawPointer) \<Longrightarrow> (valid_rawaddr p \<Longrightarrow> C) \<Longrightarrow> C"
+  unfolding Inhabited_def by (simp add: \<phi>expns)
+
+declare [[\<phi>trace_reasoning = 1]]
+
+lemma RawPointer_zero[\<phi>reason 1200]:
+  "\<phi>Zero pointer RawPointer (Null |: 0)"
+  unfolding \<phi>Zero_def by (simp add: \<phi>expns zero_prod_def zero_memaddr_def)
+
+lemma RawPointer_eqcmp[\<phi>reason 1200]:
+  "\<phi>Equal RawPointer (\<lambda>x y. x = 0 |: 0 \<or> y = 0 |: 0 \<or> memaddr.segment x = memaddr.segment y) (=)"
+  unfolding \<phi>Equal_def by (simp add: \<phi>expns zero_memaddr_def) blast
+
+lemma RawPointer_semty[\<phi>reason 1200]:
+  \<open>\<phi>SemType (x \<Ztypecolon> RawPointer) pointer\<close>
+  unfolding \<phi>SemType_def subset_iff
+  by (simp add: \<phi>expns)
+
+
+subsubsection \<open>Typed Pointer\<close>
+
+definition TypPtr :: "TY \<Rightarrow> (VAL, logaddr) \<phi>"
+  where "TypPtr TY x = ({ V_pointer.mk (logaddr_to_raw x) }
+              \<s>\<u>\<b>\<j> valid_logaddr x \<and> x \<noteq> 0 \<and> logaddr_type x = TY \<and> 0 < MemObj_Size TY)"
+
+lemma TypPtr_expn[\<phi>expns]:
+  "v \<in> (addr \<Ztypecolon> TypPtr TY) \<longleftrightarrow>
+      v = V_pointer.mk (logaddr_to_raw addr) \<and> valid_logaddr addr
+    \<and> addr \<noteq> 0 \<and> logaddr_type addr = TY \<and> 0 < MemObj_Size TY"
+  unfolding \<phi>Type_def by (simp add: TypPtr_def Subjection_expn)
+
+lemma TypPtr_inhabited[elim!, \<phi>inhabitance_rule]:
+  "Inhabited (addr \<Ztypecolon> TypPtr TY) \<Longrightarrow>
+      (valid_logaddr addr \<and> addr \<noteq> 0 \<and> logaddr_type addr = TY \<and> 0 < MemObj_Size TY \<Longrightarrow> C) \<Longrightarrow> C"
+  unfolding Inhabited_def by (simp add: \<phi>expns)
+
+lemma TypPtr_eqcmp[\<phi>reason 1000]:
+    "\<phi>Equal (TypPtr TY) (\<lambda>x y. memaddr.segment x = memaddr.segment y) (=)"
+  unfolding \<phi>Equal_def
+  by (simp add: \<phi>expns) (metis logaddr_to_raw_inj)
+
+lemma TypPtr_semty[\<phi>reason 1000]:
+  \<open>\<phi>SemType (x \<Ztypecolon> TypPtr TY) pointer\<close>
+  unfolding \<phi>SemType_def subset_iff
+  by (simp add: \<phi>expns valid_logaddr_def)
+
+subsubsection \<open>Slice Pointer\<close>
+
+text \<open>A limitation of TypPtr is that it cannot point to the end of an array,
+  because there is no object at all at the end. To address this, there is a slice pointer which
+  can range over a piece of the array including the end.\<close>
+
+definition SlicePtr :: "TY \<Rightarrow> (VAL, logaddr \<times> nat \<times> nat) \<phi>"
+  where "SlicePtr TY = (\<lambda>(base,i,len).
+    if valid_logaddr base \<and> base \<noteq> 0 \<and> (\<exists>N. logaddr_type base = array N TY \<and> len \<le> N)
+        \<and> 0 < MemObj_Size TY \<and> i \<le> len
+    then { V_pointer.mk (logaddr_to_raw base ||+ of_nat (i * MemObj_Size TY)) }
+    else {})"
+
+lemma SlicePtr_expn[\<phi>expns]:
+  \<open>v \<in> ((base, i, len) \<Ztypecolon> SlicePtr TY) \<longleftrightarrow>
+      valid_logaddr base \<and> base \<noteq> 0
+      \<and> (\<exists>N. logaddr_type base = \<tau>Array N TY \<and> len \<le> N)
+      \<and> 0 < MemObj_Size TY \<and> i \<le> len
+      \<and> v = V_pointer.mk (logaddr_to_raw base ||+ of_nat (i * MemObj_Size TY))\<close>
+  unfolding SlicePtr_def \<phi>Type_def by simp blast
+
+lemma SlicePtr_inhabited[\<phi>reason_elim!,elim!]:
+  \<open>Inhabited ((base, i, len) \<Ztypecolon> SlicePtr TY)
+\<Longrightarrow> (\<And>N. valid_logaddr base \<Longrightarrow> base \<noteq> 0 \<Longrightarrow> logaddr_type base = \<tau>Array N TY \<Longrightarrow> len \<le> N
+          \<Longrightarrow> 0 < MemObj_Size TY \<Longrightarrow> i \<le> len \<Longrightarrow> C)
+\<Longrightarrow> C\<close>
+  unfolding Inhabited_def SlicePtr_expn by simp blast
+
+lemma SlicePtr_eqcmp[\<phi>reason on \<open>\<phi>Equal (SlicePtr ?TY) ?c ?eq\<close>]:
+    "\<phi>Equal (SlicePtr TY) (\<lambda>x y. fst x = fst y) (\<lambda>(_,i1,_) (_,i2,_). i1 = i2)"
+  unfolding \<phi>Equal_def
+  apply (clarsimp simp add: \<phi>expns word_of_nat_eq_iff take_bit_nat_def simp del: of_nat_mult)
+  subgoal premises for addr i1 n1 i2 N n2 proof -
+    note logaddr_storable_in_mem[OF \<open>valid_logaddr addr\<close> \<open>addr \<noteq> 0\<close>,
+            unfolded \<open>logaddr_type addr = \<tau>Array N TY\<close>, unfolded memobj_size_arr]
+    then have \<open>i1 * MemObj_Size TY < 2 ^ addrspace_bits\<close>
+          and \<open>i2 * MemObj_Size TY < 2 ^ addrspace_bits\<close>
+      by (meson \<open>i1 \<le> n1\<close> \<open>n1 \<le> N\<close> \<open>i2 \<le> n2\<close> \<open>n2 \<le> N\<close> dual_order.strict_trans2 mult_le_mono1)+
+    then show ?thesis
+      using \<open>0 < MemObj_Size TY\<close> by fastforce 
+  qed
+  done
+
+lemma SlicePtr_semty[\<phi>reason on \<open>\<phi>SemType (?x \<Ztypecolon> SlicePtr ?TY) ?ty\<close>]:
+  \<open>\<phi>SemType (x \<Ztypecolon> SlicePtr TY) \<tau>Pointer\<close>
+  unfolding \<phi>SemType_def subset_iff
+  by (cases x, simp add: \<phi>expns valid_logaddr_def)
+
+
+
+subsection \<open>Memory Object\<close>
+
+definition (in agmem) Ref :: \<open>('VAL,'a) \<phi> \<Rightarrow> ('FIC_N \<Rightarrow> 'FIC, 'TY logaddr \<Zinj> 'a share) \<phi>\<close>
+  where \<open>Ref T x' = (case x' of (seg |: idx) \<Zinj> (n \<Znrres> x) \<Rightarrow>
+    if 0 < n \<and> valid_index (segidx.layout seg) idx then
+    { FIC_mem.mk (1(seg := Fine (push_map idx (share n (to_share o Mapof_Val v)))))
+          |v. v \<in> Well_Type (logaddr_type (seg |: idx)) \<and> v \<in> (x \<Ztypecolon> T) }
+    else {})\<close>
+
+lemma (in agmem) Ref_expn[\<phi>expns]:
+  \<open>fic \<in> ((seg |: idx) \<Zinj> (n \<Znrres> v) \<Ztypecolon> Ref Identity)
+    \<longleftrightarrow> 0 < n \<and> valid_index (segidx.layout seg) idx
+        \<and> v \<in> Well_Type (logaddr_type (seg |: idx))
+        \<and> fic = FIC_mem.mk (1(seg := Fine (push_map idx (share n (to_share o Mapof_Val v)))))\<close>
+  unfolding Ref_def \<phi>Type_def by (simp add: Identity_def) blast
+
+(*
+definition Slice :: \<open>('VAL,'a) \<phi> \<Rightarrow> ('FIC_N \<Rightarrow> 'FIC, 'TY logaddr \<Zinj> 'a share option list) \<phi>\<close>
+  where \<open>Slice T x' = (case x' of (seg |: i#idx) \<Zinj> l \<Rightarrow>
+    if valid_index (segidx.layout seg) idx
+     \<and> (\<exists>N TY. index_type idx (segidx.layout seg) = \<tau>Array N TY \<and> i + length l \<le> N)
+    then let 
+    { FIC_mem.mk (1(seg := Fine (push_map idx (share n (to_share o Mapof_Val v)))))
+          |v. v \<in> Well_Type (logaddr_type (seg |: idx)) \<and> v \<in> (x \<Ztypecolon> T) }
+    else {} | _ \<Rightarrow> {})\<close> *)
+
+section \<open>Instructions & Their Specifications\<close>
+
+
+
+subsubsection \<open>Address / Pointer\<close>
+
+definition \<phi>M_get_logptr :: \<open>'TY \<Rightarrow> 'VAL sem_value \<Rightarrow> ('TY logaddr \<Rightarrow> ('ret,'RES_N,'RES) proc) \<Rightarrow> ('ret,'RES_N,'RES) proc\<close>
+  where \<open>\<phi>M_get_logptr TY v F = \<phi>M_getV \<tau>Pointer V_pointer.dest v (\<lambda>p. F (rawaddr_to_log TY p))\<close>
+
+lemma (in agmem) \<phi>M_get_logptr[\<phi>reason!]:
+  \<open>(valid_logaddr addr \<Longrightarrow>
+    addr \<noteq> 0 \<Longrightarrow>
+    logaddr_type addr = TY \<Longrightarrow>
+    0 < MemObj_Size TY \<Longrightarrow>
+    \<^bold>p\<^bold>r\<^bold>o\<^bold>c F addr \<lbrace> X \<longmapsto> Y \<rbrace>) \<Longrightarrow>
+   \<^bold>p\<^bold>r\<^bold>o\<^bold>c \<phi>M_get_logptr TY v F \<lbrace> X\<heavy_comma> addr \<Ztypecolon> Val v (Pointer TY) \<longmapsto> Y \<rbrace>\<close>
+  unfolding \<phi>M_get_logptr_def
+  by (cases v, simp, rule \<phi>M_getV, simp add: \<phi>expns valid_logaddr_def, auto simp add: \<phi>expns)
+
+
+subsection \<open>Access the Resource\<close>
+
+subsubsection \<open>Memory Operations\<close>
+
+definition \<phi>M_get_mem
+    :: "'TY segidx \<Rightarrow> nat list \<Rightarrow> ('VAL \<Rightarrow> ('ret,'RES_N,'RES) proc) \<Rightarrow> ('ret,'RES_N,'RES) proc"
+  where "\<phi>M_get_mem seg idx F =
+            \<phi>M_get_res_entry R_mem.get seg (\<lambda>val.
+            \<phi>M_assert (val \<in> Well_Type (segidx.layout seg)) \<ggreater> F (index_value idx val))"
+
+definition op_load_mem :: "'TY \<Rightarrow> ('VAL, 'VAL,'RES_N,'RES) proc'"
+  where "op_load_mem TY v =
+    \<phi>M_get_logptr TY v (\<lambda>ptr.
+    \<phi>M_get_mem (memaddr.segment ptr) (memaddr.index ptr) (\<lambda>x. Return (sem_value x)))"
+
+definition op_store_mem :: "'TY \<Rightarrow> ('VAL \<times> 'VAL, unit,'RES_N,'RES) proc'"
+  where "op_store_mem TY =
+    \<phi>M_caseV (\<lambda>va vb.
+    \<phi>M_get_logptr TY va (\<lambda>ptr. case ptr of (seg |: idx) \<Rightarrow>
+    \<phi>M_getV TY id vb (\<lambda>v.
+    \<phi>M_get_mem seg idx (\<lambda>_.
+    \<phi>M_set_res R_mem.updt (\<lambda>f. f(seg := map_option (index_mod_value idx (\<lambda>_. v)) (f seg)))))))"
+
+definition op_free_mem :: "('VAL, unit,'RES_N,'RES) proc'"
+  where "op_free_mem v =
+    \<phi>M_getV \<tau>Pointer V_pointer.dest v (\<lambda>ptr. case ptr of (seg |: ofst) \<Rightarrow>
+    \<phi>M_assert (ofst = 0) \<ggreater>
+    \<phi>M_set_res R_mem.updt (\<lambda>f. f(seg := None)))"
+
+definition op_alloc_mem :: "'TY \<Rightarrow> ('VAL, unit,'RES_N,'RES) proc'"
+  where "op_alloc_mem TY' v =
+    \<phi>M_getV (\<tau>Int addrspace_bits) V_int.dest v (\<lambda>(_, n).
+    \<phi>M_set_res R_mem.updt (\<lambda>f.
+    let TY = \<tau>Array n TY'
+      ; addr = (@addr. f addr = None \<and> segidx.layout addr = TY)
+     in f(addr := Some (Zero TY))))"
+
+declare (in agmem) fiction_mem_\<I>[simp]
+
+lemma (in agmem) \<phi>M_get_mem[\<phi>reason!]:
+  \<open>\<^bold>p\<^bold>r\<^bold>o\<^bold>c F v \<lbrace> (seg |: idx) \<Zinj> n \<Znrres> v \<Ztypecolon> Ref Identity \<longmapsto> Y \<rbrace>
+    \<Longrightarrow> \<^bold>p\<^bold>r\<^bold>o\<^bold>c \<phi>M_get_mem seg idx F \<lbrace> (seg |: idx) \<Zinj> n \<Znrres> v \<Ztypecolon> Ref Identity \<longmapsto> Y \<rbrace>\<close>
+  unfolding \<phi>Procedure_def
+  apply clarify
+  apply (subgoal_tac \<open>\<phi>M_get_mem seg idx F comp = F v comp\<close>)
+  apply simp
+  unfolding \<phi>M_get_mem_def \<phi>M_get_res_entry_def \<phi>M_get_res_def
+  apply (auto simp add: \<phi>expns FIC_mem.interp_split' R_mem_valid_split' share_mem_def
+                R_mem.mult_in_dom Valid_Mem_def times_fun
+                mult_strip_fine_011 times_list_def del: subsetI)
+  subgoal premises prems for R fic res mem mem'
+  proof -
+    note [simp] = mult_strip_fine_011
+    from \<open>mem' ## mem\<close> have t1: \<open>mem' seg ## mem seg\<close> by (simp add: sep_disj_fun) 
+    show ?thesis
+      using \<open>\<forall>_. \<exists>_. _ = Fine _ \<and> _ \<in> _\<close>[THEN spec[where x=seg]] t1 \<open>valid_index (segidx.layout seg) idx\<close>
+        apply (auto simp add: \<open>0 < n\<close>)
+      using \<open>\<forall>_ \<in> dom _. _\<close>[unfolded Ball_def, THEN spec[where x=seg]]
+       apply (auto simp add: times_fun)[1]
+
+      subgoal premises prems2 for sh' v' proof -
+        have [simp]: \<open>valid_index (segidx.layout seg) idx\<close>
+          by (simp add: \<open>valid_index (segidx.layout seg) idx\<close> \<open>v' \<in> Well_Type (segidx.layout seg)\<close>)
+        note t2[simp] = this[THEN Mapof_Val_pull]
+
+        have t3[simp]: \<open>pull_map idx sh' ## share n (to_share \<circ> Mapof_Val v)\<close>
+          using \<open>sh' ## push_map idx _\<close> by (metis pull_map_sep_disj pull_push_map)
+        have t5: \<open>index_value idx v' \<in> Well_Type (index_type idx (segidx.layout seg))\<close>
+          using index_value_welltyp \<open>valid_index (segidx.layout seg) idx\<close>
+                  \<open>v' \<in> Well_Type (segidx.layout seg)\<close> by blast
+
+        let \<open>?lhs = ?rhs\<close> = \<open>to_share \<circ> Mapof_Val v' = sh' * push_map idx (share n (to_share \<circ> Mapof_Val v))\<close>
+        from \<open>?lhs = ?rhs\<close> have \<open>pull_map idx ?lhs = pull_map idx ?rhs\<close> by fastforce
+        note this[simplified pull_map_to_share pull_map_homo_mult pull_push_map t2]
+        then have \<open>Mapof_Val (index_value idx v') = (strip_share \<circ> pull_map idx sh') ++ (Mapof_Val v)\<close>
+          by (metis prems(5) prems2(6) strip_share_fun_mult strip_share_fun_share strip_share_share_funcomp(2) t2 t3)
+        then have txx: \<open>index_value idx v' = v\<close>
+          using Valof_Map_append Valof_Map t5
+          by (metis prems(7))
+        
+        show ?thesis by (subst txx) standard
+      qed
+      done
+  qed
+  done
+
+lemma (in agmem) op_load_mem:
+  \<open>\<^bold>p\<^bold>r\<^bold>e\<^bold>m\<^bold>i\<^bold>s\<^bold>e v \<in> Well_Type TY
+    \<Longrightarrow> \<^bold>p\<^bold>r\<^bold>o\<^bold>c op_load_mem TY raw
+          \<lbrace> ptr \<Zinj> n \<Znrres> v \<Ztypecolon> Ref Identity\<heavy_comma> ptr \<Ztypecolon> Val raw (Pointer TY) \<longmapsto> ptr \<Zinj> n \<Znrres> v \<Ztypecolon> Ref Identity\<heavy_comma> \<^bold>v\<^bold>a\<^bold>l v \<Ztypecolon> Identity \<rbrace>\<close>
+  unfolding Premise_def op_load_mem_def
+  apply (cases ptr; simp)
+  apply \<phi>reason
+  apply simp
+  by \<phi>reason
+
+lemma (in agmem) op_store_mem:
+   \<open>\<^bold>p\<^bold>r\<^bold>e\<^bold>m\<^bold>i\<^bold>s\<^bold>e v \<in> Well_Type TY
+\<Longrightarrow> \<^bold>p\<^bold>r\<^bold>e\<^bold>m\<^bold>i\<^bold>s\<^bold>e u \<in> Well_Type TY
+\<Longrightarrow> \<^bold>p\<^bold>r\<^bold>o\<^bold>c op_store_mem TY (\<phi>V_pair raw_ptr raw_u)
+          \<lbrace> ptr \<Zinj> 1 \<Znrres> v \<Ztypecolon> Ref Identity\<heavy_comma> u \<Ztypecolon> Val raw_u Identity\<heavy_comma> ptr \<Ztypecolon> Val raw_ptr (Pointer TY)
+        \<longmapsto> ptr \<Zinj> 1 \<Znrres> u \<Ztypecolon> Ref Identity\<rbrace>\<close>
+  unfolding Premise_def op_store_mem_def
+  apply (rule \<phi>M_caseV, rule \<phi>M_get_logptr)
+  apply (cases ptr; cases raw_u; simp, \<phi>reason)
+  unfolding \<phi>M_set_res_def \<phi>Procedure_def
+  apply (auto simp add: \<phi>expns FIC_mem.interp_split' R_mem_valid_split' share_mem_def
+                        R_mem.mult_in_dom times_list_def)
+  subgoal premises prems for seg idx R fic res mem mem_remain'
+  proof -
+    show ?thesis
+      using \<open>\<forall>_. \<exists>_. _ \<and> mem _ \<in> _\<close>[THEN spec[where x=seg]] \<open>mem_remain' * Fine mem \<in> Valid_Mem\<close>
+      apply (auto simp add: mult_strip_fine_011 prems Valid_Mem_def times_fun
+                            sep_disj_partial_map_some_none times_fine times_list_def)
+      subgoal premises prems2 for fic_mR mem_R val
+      proof -
+        have [simp]: \<open>seg \<in> dom mem\<close> using \<open>mem seg = Some val\<close> by blast
+        have [simp]: \<open>\<And>any. mem_R ## mem(seg := any)\<close> using \<open>mem_R ## _\<close> \<open>mem seg = Some val\<close>
+          by (smt (verit, best) fun_upd_apply sep_disj_commuteI sep_disj_fun_def sep_disj_option(3) sep_disj_partial_map_some_none)
+      have t1: \<open>dom (push_map idx (to_share \<circ> Mapof_Val u)) = dom (push_map idx (to_share \<circ> Mapof_Val v))\<close>
+        by simp (meson Mapof_Val_same_dom \<open>u \<in> Well_Type _\<close> \<open>v \<in> Well_Type _\<close>)
+      have t2: \<open>fic_mR ## push_map idx (to_share \<circ> Mapof_Val u)\<close>
+        using total_Mapof_disjoint dom1_disjoint_sep_disj dom1_dom t1
+        by (metis \<open>fic_mR ## _\<close> \<open>to_share \<circ> Mapof_Val val = _\<close>)
+        
+        show ?thesis
+          apply (rule exI[where x=\<open>fic * FIC_mem.mk (1(seg := Fine (push_map idx (to_share \<circ> Mapof_Val u))))\<close>])
+          apply (auto simp add: prems prems2 inj_image_mem_iff index_mod_value_welltyp
+                                FIC_mem.interp_split' R_mem.times_fun_upd sep_disj_partial_map_upd
+                                times_set_def times_fine'[symmetric] R_mem.mk_homo_mult)
+          apply (fold \<open>mem_remain' = Fine mem_R\<close>,
+                 fold \<open>res R_mem.name = R_mem.inject mem_remain'\<close>,
+                 fold mult.assoc,
+                 fold R_mem.split)
+          apply (rule exI[where x=\<open>res\<close>])
+          apply (rule exI[where x=\<open>R_mem.mk (Fine (mem(seg \<mapsto> index_mod_value idx (\<lambda>_. u) val)))\<close>])
+          apply (simp add: prems share_mem_def )
+          apply (auto simp add: mult_strip_fine_011 times_fun inj_image_mem_iff prems2 times_fine t2)
+          apply (rule exI[where x =\<open>fic_mR * push_map idx (to_share \<circ> Mapof_Val u)\<close>],
+              simp add: Mapof_Val_modify_fiction[of \<open>segidx.layout seg\<close> idx val v u fic_mR]
+                        prems2 prems index_mod_value_welltyp)
+          subgoal for x
+            using \<open>\<forall>_. \<exists>y. _\<close>[THEN spec[where x=x]] apply clarsimp apply (case_tac \<open>y=1\<close>; simp)
+          subgoal for y by (rule exI[where x=y], simp)
+          done
+        done
+    qed
+    done
+  qed
+  done
+
+
+declare (in agmem) fiction_mem_\<I>[simp del]
+
+
+lemma (in agmem) fiction_mem_\<I>':
+  \<open> Rmem \<in> \<I> (fiction_mem (fiction.defined I)) fic
+\<longleftrightarrow> (\<exists>mem. Rmem = R_mem.mk (Fine mem) \<and> mem \<in> \<I> I fic)\<close>
+  unfolding fiction_mem_\<I> by clarsimp blast
+
+lemma (in agmem) fiction_mem_\<I>'':
+  \<open> Rmem R_mem.name = R_mem.inject (Fine mem)
+\<Longrightarrow> Rmem \<in> \<I> (fiction_mem (fiction.defined I)) fic
+\<longleftrightarrow> Rmem = R_mem.mk (Fine mem) \<and> mem \<in> \<I> I fic\<close>
+  unfolding fiction_mem_\<I>' by auto
+
+lemma (in agmem) fiction_mem_\<I>_simp:
+  \<open> R_mem.mk (Fine mem) \<in> \<I> (fiction_mem (fiction.defined I)) fic
+\<longleftrightarrow> mem \<in> \<I> I fic\<close>
+  unfolding fiction_mem_\<I>' by simp
+
+
+
+lemma (in agmem) share_mem_in_dom:
+  \<open> mem \<in> \<I> share_mem' fic
+\<Longrightarrow> seg \<in> dom1 fic
+\<Longrightarrow> seg \<in> dom mem\<close>
+  unfolding share_mem'_def
+  by (simp add: domIff dom1_def one_fine_def)
+     (smt (verit, ccfv_SIG) mem_Collect_eq option.distinct(1))
+
+
+lemma (in agmem) share_mem'_mono:
+  \<open> x \<in> \<I> share_mem' fx
+\<Longrightarrow> y \<in> \<I> share_mem' fy
+\<Longrightarrow> dom1 fx \<inter> dom1 fy = {}
+\<Longrightarrow> x * y \<in> \<I> share_mem' (fx * fy)\<close>
+  unfolding share_mem'_def set_eq_iff
+  apply clarsimp
+  subgoal premises prems for k
+    using prems[THEN spec[where x=k]]
+  apply (clarsimp simp add: times_fun dom1_def one_fine_def)
+    subgoal for fx' fy'
+      apply (cases \<open>fx' = 1\<close>; cases \<open>fy' = 1\<close>; clarsimp simp add: times_fine)
+      using Mapof_not_1 to_share_funcomp_eq_1_iff by blast+
+    done
+  done
+
+
+
+lemma (in agmem) share_mem'_drop_seg:
+  \<open> v \<in> Well_Type (segidx.layout seg)
+\<Longrightarrow> mem \<in> \<I> share_mem' (fic * 1(seg := Fine (to_share \<circ> Mapof_Val v)))
+\<Longrightarrow> seg \<in> dom mem \<and> mem(seg := None) \<in> \<I> share_mem' fic\<close>
+  unfolding share_mem'_def
+  apply (auto simp add: times_fun)
+  subgoal premises prems proof -
+    show ?thesis
+      using prems(2)[THEN spec[where x=seg]]
+      by (clarsimp simp add: mult_strip_fine_011)
+  qed
+  subgoal premises prems proof -
+    show ?thesis
+      using prems(2)[THEN spec[where x=seg]]
+      apply (clarsimp simp add: mult_strip_fine_011)  
+      subgoal premises prems2 for r u proof -
+        have \<open>dom r \<inter> dom (to_share o Mapof_Val v) = {}\<close>
+          using total_Mapof_disjoint[where idx=\<open>[]\<close>, simplified]
+                \<open>r ## (to_share \<circ> Mapof_Val v)\<close> \<open>to_share \<circ> Mapof_Val u = r * (to_share \<circ> Mapof_Val v)\<close>
+          by fastforce
+        moreover have \<open>dom (to_share \<circ> Mapof_Val u) = dom (to_share \<circ> Mapof_Val v)\<close>
+          using Mapof_Val_same_dom
+          by (metis \<open>u \<in> Well_Type (segidx.layout seg)\<close> dom_map_option_comp prems(1)) 
+        moreover have \<open>dom (to_share \<circ> Mapof_Val u) = dom r \<union> dom (to_share \<circ> Mapof_Val v)\<close>
+          using dom_mult by (metis prems2) 
+        ultimately have \<open>dom r = {}\<close> by (metis inf_sup_absorb)
+        then show ?thesis unfolding one_partial_map by blast
+      qed
+      done
+  qed
+  subgoal premises prems for x proof -
+    thm prems
+    show ?thesis using \<open>\<forall>_. _\<close>[THEN spec[where x=x]] \<open>x\<noteq>seg\<close> apply clarsimp
+      subgoal for m by (rule exI[where x=m], simp, cases \<open>m = 1\<close>; simp)
+      done
+  qed
+  done
+
+
+lemma (in agmem) op_alloc_mem:
+  \<open>\<^bold>p\<^bold>r\<^bold>o\<^bold>c op_alloc_mem TY raw_n \<lbrace> n \<Ztypecolon> Val raw_n Size \<longmapsto> ((seg |: []) \<Zinj> 1 \<Znrres> (Zero (\<tau>Array n TY)) \<Ztypecolon> Ref Identity \<^bold>s\<^bold>u\<^bold>b\<^bold>j seg. True) \<rbrace>\<close>
+  unfolding op_alloc_mem_def
+  apply (cases raw_n; simp, rule \<phi>M_tail_left, rule \<phi>M_getV; simp add: \<phi>expns)
+  unfolding \<phi>M_set_res_def \<phi>Procedure_def
+  apply (auto simp add: \<phi>expns FIC_mem.interp_split' R_mem_valid_split' times_fun dom_mult
+                        R_mem.mult_in_dom Valid_Mem_def mult_strip_fine_011 mult_strip_fine_001
+                        fiction_mem_\<I>'' share_mem_def' times_list_def)
+  subgoal premises prems for R fic res mem' mem
+  proof -
+    note [simp] = times_fun dom_mult
+    have t0: \<open>finite (dom (mem' * mem))\<close> using prems by simp
+    note t1 = Mem_freshness[OF t0, of \<open>\<tau>Array n TY\<close>, THEN someI_ex, simplified]
+    let ?seg = \<open>(SOME x. mem' x = None \<and> mem x = None \<and> segidx.layout x = \<tau>Array n TY)\<close>
+    have t2'[simp]: \<open>mem' ?seg = None \<and> mem ?seg = None\<close> using t1 by blast
+    have t2'': \<open>?seg \<notin> dom mem\<close> by force
+    have t6: \<open>\<And>any. R_mem.clean res * R_mem.mk (Fine ((mem' * mem)(?seg := any)))
+                  = res * (R_mem.mk (Fine (mem * 1(?seg := any))))\<close>
+      unfolding fun_upd_def fun_eq_iff
+      apply (simp add: prems R_mem.inj_homo_mult[symmetric] times_fine fun_eq_iff sep_disj_fun_def)
+      by (simp add: \<open>mem' ## mem\<close> sep_disj_fun)
+
+    show ?thesis
+      apply (rule exI[where x = \<open>fic * FIC_mem.mk
+                  (1(?seg := Fine (to_share \<circ> Mapof_Val (V_array.mk (TY, replicate n (Zero TY))))))\<close>])
+      apply (auto simp add: prems inj_image_mem_iff t1 list_all_length zero_well_typ
+                            FIC_mem.interp_split' R_mem.times_fun_upd sep_disj_partial_map_upd
+                            times_set_def times_fine'[symmetric] R_mem.mk_homo_mult)
+       apply (rule exI[where x=\<open>?seg\<close>], rule exI[where x=fic], simp add: prems t1 list_all_length zero_well_typ)
+      apply (unfold t6)
+      apply (rule exI[where x=\<open>res\<close>])
+      apply (rule exI[where x=\<open>R_mem.mk (Fine (mem * 1(?seg \<mapsto> V_array.mk (TY, replicate n (Zero TY)))))\<close>])
+      using \<open>res \<in> \<I> INTERP (FIC_mem.clean fic)\<close>
+      apply (clarsimp simp add: prems share_mem_def' fiction_mem_\<I>_simp)
+      apply (rule share_mem'_mono, simp add: prems)
+      apply (clarsimp simp add: share_mem'_def t1 list_all_length zero_well_typ one_fine_def)
+      apply (simp add: set_eq_iff)
+      using share_mem_in_dom[OF \<open>mem \<in> \<I> share_mem' (FIC_mem.get fic)\<close>]  t2'' by blast
+  qed
+  done
+
+
+lemma (in agmem) op_free_mem:
+   \<open>\<^bold>p\<^bold>r\<^bold>o\<^bold>c op_free_mem vptr \<lbrace> (seg |: []) \<Zinj> 1 \<Znrres> v \<Ztypecolon> Ref Identity\<heavy_comma> (seg |: 0) \<Ztypecolon> Val vptr RawPointer \<longmapsto> 1\<rbrace>\<close>
+  unfolding op_free_mem_def
+  apply (cases vptr; simp, rule \<phi>M_getV; simp add: \<phi>expns)
+  unfolding \<phi>M_set_res_def \<phi>Procedure_def
+  apply (auto simp add: \<phi>expns FIC_mem.interp_split' R_mem_valid_split' times_fun dom_mult
+                        R_mem.mult_in_dom Valid_Mem_def mult_strip_fine_011 mult_strip_fine_001
+                        fiction_mem_\<I>'' share_mem_def' times_list_def)
+  subgoal premises prems for R fic res memR mem
+  proof -
+    have t2: \<open>seg \<in> dom mem\<close>
+      using share_mem'_drop_seg prems by blast 
+    have t3: \<open>seg \<notin> dom memR\<close>
+      by (meson domD domIff prems sep_disj_partial_map_some_none t2)
+    have t1: \<open>(res * R_mem.mk (Fine mem))(R_mem.name := R_mem.inject (Fine ((memR * mem)(seg := None))))
+            = res * R_mem.mk (Fine (mem(seg := None)))\<close>
+      unfolding fun_eq_iff times_fun
+      apply (simp add: prems R_mem.inj_homo_mult[symmetric] times_fine sep_disj_partial_map_del)
+      apply (simp add: fun_upd_def fun_eq_iff times_fun)
+      using domIff t3 by fastforce
+    show ?thesis
+      apply (rule exI[where x=fic], simp add: prems FIC_mem.interp_split' sep_disj_partial_map_del t1)
+      apply (rule times_set_I, simp add: prems)
+      using share_mem'_drop_seg prems
+      by (metis fiction_mem_\<I>' share_mem_def')
+  qed
+  done
+
+
+
+end
+
+
+
+
+
+
+end
