Phi_Semantics/PhiSem_Mem_C_Array.thy
@@ -1,0 +1,10 @@
+theory PhiSem_Mem_C_Array
+  imports PhiSem_Mem_C_Base PhiSem_Aggregate_Array
+begin
+
+debt_axiomatization
+    memobj_size_arr: \<open>MemObj_Size (array N T) = N * MemObj_Size T\<close>
+and Mapof_Val_arr: \<open>Mapof_Val (V_array.mk vs) = nnode (map Mapof_Val vs)\<close>
+
+
+end
