Phi_Semantics/PhiSem_Mem_C_Base.thy
@@ -1,0 +1,181 @@
+theory PhiSem_Mem_C_Base
+  imports PhiSem_Aggregate_Base
+begin
+
+section \<open>Semantics\<close>
+
+debt_axiomatization
+        MemObj_Size :: \<open>TY \<Rightarrow> nat\<close>
+    and idx_step_offset :: \<open>TY \<Rightarrow> nat \<Rightarrow> nat\<close>
+  where memobj_size_step : \<open>valid_idx_step T i \<Longrightarrow> MemObj_Size (idx_step_type i T) \<le> MemObj_Size T\<close>
+    and idx_step_offset_size:
+          \<open>valid_idx_step T i
+                \<Longrightarrow> idx_step_offset T i + MemObj_Size (idx_step_type i T) \<le> MemObj_Size T\<close>
+    and idx_step_offset_disj:
+          \<open>valid_idx_step T i \<Longrightarrow> valid_idx_step T j \<Longrightarrow>
+                idx_step_offset T i \<le> idx_step_offset T j \<Longrightarrow>
+                idx_step_offset T j < idx_step_offset T i + MemObj_Size (idx_step_type i T) \<Longrightarrow>
+                i = j\<close>
+
+primrec index_offset :: \<open>TY \<Rightarrow> nat list \<Rightarrow> nat\<close>
+  where \<open>index_offset T [] = 0\<close>
+      | \<open>index_offset T (i#idx) = idx_step_offset T i + index_offset (idx_step_type i T) idx\<close>
+
+lemma index_offset_tail[simp]:
+  \<open>index_offset T (idx@[i]) = index_offset T idx + idx_step_offset (index_type idx T) i\<close>
+  by (induct idx arbitrary: T; simp)
+
+lemma fold_tail:
+  \<open>fold f (l @ [x]) = f x o fold f l\<close>
+  by (induct l; simp)
+
+lemma index_offset_upper_bound:
+  \<open>valid_index T (base@idx) \<Longrightarrow>
+   index_offset T (base@idx) + MemObj_Size (index_type (base@idx) T) \<le> index_offset T base + MemObj_Size (index_type base T)\<close>
+  apply (induct idx arbitrary: base rule: rev_induct;
+         simp del: append_assoc add: append_assoc[symmetric] fold_tail)
+  using idx_step_offset_size by fastforce
+
+lemmas index_offset_upper_bound_0 = index_offset_upper_bound[where base = "[]", simplified]
+
+lemma index_offset_bound:
+  \<open>valid_index T (base@idx) \<Longrightarrow>
+  index_offset T base \<le> index_offset T (base@idx) \<and> index_offset T (base@idx) \<le> index_offset T base + MemObj_Size (index_type base T)\<close>
+  apply (induct idx arbitrary: base rule: rev_induct;
+         simp del: append_assoc add: append_assoc[symmetric] fold_tail)
+  using idx_step_offset_size index_offset_upper_bound by fastforce
+
+lemma index_offset_bound_strict:
+  \<open>valid_index T (base@idx) \<Longrightarrow> 0 < MemObj_Size (index_type (base@idx) T) \<Longrightarrow>
+  index_offset T base \<le> index_offset T (base@idx) \<and> index_offset T (base@idx) < index_offset T base + MemObj_Size (index_type base T)\<close>
+  apply (induct idx arbitrary: base rule: rev_induct;
+         simp del: append_assoc add: append_assoc[symmetric] fold_tail)
+  using idx_step_offset_size index_offset_upper_bound by fastforce
+
+
+section \<open>Fiction\<close>
+
+debt_axiomatization Mapof_Val :: \<open>VAL \<Rightarrow> nat list \<rightharpoonup> VAL\<close>
+  where Mapof_Val_inj: \<open>Va \<in> Well_Type T \<Longrightarrow> Vb \<in> Well_Type T \<Longrightarrow> Mapof_Val Va = Mapof_Val Vb \<Longrightarrow> Va = Vb\<close>
+  and   Mapof_Val_same_dom: \<open>Va \<in> Well_Type T \<Longrightarrow> Vb \<in> Well_Type T \<Longrightarrow> dom (Mapof_Val Va) = dom (Mapof_Val Vb)\<close>
+  and   Mapof_not_1[simp]: \<open>Mapof_Val V \<noteq> 1\<close>
+  and   Mapof_Val_pull_step: \<open>valid_idx_step T i \<Longrightarrow> V \<in> Well_Type T
+                          \<Longrightarrow> pull_map [i] (Mapof_Val V) = Mapof_Val (idx_step_value i V)\<close>
+  and   Mapof_Val_mod_step: \<open>valid_idx_step T i \<Longrightarrow> v \<in> Well_Type T
+                         \<Longrightarrow> Mapof_Val (idx_step_mod_value i f v) = Mapof_Val v ++ push_map [i] (Mapof_Val (f (idx_step_value i v)))\<close>
+
+lemma Mapof_Val_pull:
+  \<open>valid_index T idx \<Longrightarrow> V \<in> Well_Type T \<Longrightarrow> pull_map idx (Mapof_Val V) = Mapof_Val (index_value idx V)\<close>
+  apply (induct idx arbitrary: V T; simp)
+  using Mapof_Val_pull_step
+  by (metis idx_step_value_welltyp pull_map_cons)
+
+lemma total_Mapof_disjoint:
+   \<open>g ## (push_map idx (to_share \<circ> h))
+\<Longrightarrow> to_share \<circ> f = g * (push_map idx (to_share \<circ> h))
+\<Longrightarrow> dom g \<inter> dom (push_map idx (to_share \<circ> h)) = {}\<close>
+  using to_share_total_disjoint push_map_to_share by metis
+
+lemma map_add_subsumed_dom:
+  \<open>dom f \<subseteq> dom g \<Longrightarrow> f ++ g = g\<close>
+  unfolding map_add_def dom_def subset_eq fun_eq_iff apply simp
+  by (metis option.case_eq_if option.collapse option.simps(3))
+
+lemma Mapof_Val_mod:
+  \<open> valid_index T idx
+\<Longrightarrow> v \<in> Well_Type T
+\<Longrightarrow> u \<in> Well_Type (index_type idx T)
+\<Longrightarrow> Mapof_Val (index_mod_value idx (\<lambda>_. u) v) = Mapof_Val v ++ push_map idx (Mapof_Val u)\<close>
+  apply (induct idx arbitrary: u v T; simp)
+  using Mapof_Val_same_dom map_add_subsumed_dom apply (metis order_refl)
+  by clarify (simp add: idx_step_value_welltyp Mapof_Val_mod_step  push_map_distrib_map_add
+                        Mapof_Val_pull_step[symmetric] push_pull_map map_add_subsumed2
+                        push_map_push_map)
+
+lemma Mapof_Val_modify_fiction:
+   \<open>valid_index T idx
+\<Longrightarrow> v \<in> Well_Type T
+\<Longrightarrow> u \<in> Well_Type (index_type idx T)
+\<Longrightarrow> u'\<in> Well_Type (index_type idx T)
+\<Longrightarrow> g ## (push_map idx (to_share \<circ> Mapof_Val u))
+\<Longrightarrow> to_share \<circ> (Mapof_Val v) = g * (push_map idx (to_share \<circ> Mapof_Val u))
+\<Longrightarrow> to_share \<circ> (Mapof_Val (index_mod_value idx (\<lambda>_. u') v)) = g * (push_map idx (to_share \<circ> Mapof_Val u'))\<close>
+  apply (simp add: Mapof_Val_mod to_share_funcomp_map_add push_map_to_share
+      times_fun_map_add_right total_Mapof_disjoint[simplified push_map_to_share]
+      Mapof_Val_same_dom push_map_dom_eq)
+  subgoal premises prems proof -
+    have \<open>dom g \<inter> dom (to_share \<circ> push_map idx (Mapof_Val u)) = {}\<close>
+      using prems to_share_total_disjoint by blast
+    moreover have t1:
+      \<open>dom (to_share \<circ> push_map idx (Mapof_Val u)) = dom (to_share \<circ> push_map idx (Mapof_Val u'))\<close>
+      using prems by (metis Mapof_Val_same_dom dom_map_option_comp push_map_dom_eq)
+    ultimately have \<open>dom g \<inter> dom (to_share \<circ> push_map idx (Mapof_Val u')) = {}\<close> by metis
+    note [simp] = times_fun_map_add_right[OF this]
+    show ?thesis by simp (metis t1 map_add_subsumed_dom order_eq_refl)
+  qed
+  done
+(* lemma pull_map_share_Mapof_not_eq_1[simp]:
+  \<open>valid_index (Typeof v) idx \<Longrightarrow> pull_map idx (share n (to_share \<circ> Mapof_Val v)) = 1 \<longleftrightarrow> n = 0\<close>
+  by (cases \<open>n = 0\<close>; simp add: pull_map_share pull_map_to_share Mapof_Val_pull)
+*)
+
+
+lemma map_add_restrict_itself [simp]: \<open>(f ++ g) |` dom g = g\<close>
+  unfolding fun_eq_iff restrict_map_def map_add_def
+  by (simp add: domIff option.case_eq_if)
+
+lemma Mapof_Val_inj_plus:
+  \<open>Va \<in> Well_Type T \<Longrightarrow> Vb \<in> Well_Type T \<Longrightarrow> f ++ Mapof_Val Va = f ++ Mapof_Val Vb \<Longrightarrow> Va = Vb\<close>
+proof (rule Mapof_Val_inj, assumption)
+  assume tyA: \<open>Va \<in> Well_Type T\<close>
+     and tyB: \<open>Vb \<in> Well_Type T\<close>
+     and feq: \<open>f ++ Mapof_Val Va = f ++ Mapof_Val Vb\<close>
+  then have \<open>(f ++ Mapof_Val Va) |` dom (Mapof_Val Va) = (f ++ Mapof_Val Vb) |` dom (Mapof_Val Vb)\<close>
+    using Mapof_Val_same_dom by metis 
+  note this [simplified]
+  then show \<open>Mapof_Val Va = Mapof_Val Vb\<close> .
+qed
+
+definition \<open>Valof_Map TY M = (@V. (\<exists>f. f ++ Mapof_Val V = M) \<and> V \<in> Well_Type TY)\<close>
+
+lemma Valof_Map_append[simp]:
+  \<open>v \<in> Well_Type T \<Longrightarrow> Valof_Map T (f ++ Mapof_Val v) = v\<close>
+  unfolding Valof_Map_def
+  using someI[where P=\<open>\<lambda>V. (\<exists>fa. fa ++ Mapof_Val V = f ++ Mapof_Val v) \<and> V \<in> Well_Type T\<close> and x=v, simplified]
+        Mapof_Val_inj_plus
+  by (metis (no_types, lifting) Mapof_Val_same_dom map_add_restrict_itself) 
+
+lemmas Valof_Map[simp] = Valof_Map_append[where f = \<open>Map.empty\<close>, simplified]
+
+
+definition \<open>fic_val_to_share_map TY =
+      Interp (\<lambda>m. if m = 1 then {None} else {Some v |v. v \<in> Well_Type TY \<and> to_share o Mapof_Val v = m})\<close>
+
+lemma fic_val_to_share_map[simp]:
+  \<open>\<I> (fic_val_to_share_map TY) = (\<lambda>m. if m = 1 then {None} else {Some v |v. v \<in> Well_Type TY \<and> to_share o Mapof_Val v = m})\<close>
+  unfolding fic_val_to_share_map_def by (rule Interp_inverse) (simp add: Interpretation_def one_set_def)
+
+
+paragraph \<open>Basic fictions for resource elements\<close>
+
+definition "fiction_mem I = Fiction (\<lambda>x. { 1(R_mem #= y) |y. y \<in> \<I> I x})"
+lemma fiction_mem_\<I>:
+  "\<I> (fiction_mem I) = (\<lambda>x. { 1(R_mem #= y) |y. y \<in> \<I> I x})"
+  unfolding fiction_mem_def
+  by (rule Fiction_inverse) (auto simp add: Fictional_def one_set_def)
+
+
+
+definition "share_mem' = 
+              fiction.pointwise' (\<lambda>seg. fiction.fine (share_val_fiction (segidx.layout seg)))"
+
+definition "share_mem = fiction_mem (fiction.defined (
+              fiction.pointwise' (\<lambda>seg. fiction.fine (share_val_fiction (segidx.layout seg)))))"
+
+lemma share_mem_def':
+  \<open>share_mem = fiction_mem (fiction.defined share_mem')\<close>
+  unfolding share_mem_def share_mem'_def ..
+
+
+
+end
