Phi_Semantics/PhiSem_Mem_C_Tuple.thy
@@ -1,0 +1,9 @@
+theory PhiSem_Mem_C_Tuple
+  imports PhiSem_Mem_C_Base PhiSem_Aggregate_Tuple
+begin
+
+debt_axiomatization
+    Mapof_Val_tup: \<open>Mapof_Val (V_tup.mk vs) = nnode (map Mapof_Val vs)\<close>
+
+
+end
