Phi_Semantics/PhiSem_Variable.thy
@@ -382,19 +382,19 @@ proc op_var_scope:
 subsection \<open>Implementing IDE-CP Generic Variable Access\<close>
 
 lemma "__set_var_rule__":
-  \<open> \<p>\<r>\<o>\<c> g \<lbrace> R\<heavy_comma> y \<Ztypecolon> \<v>\<a>\<r>[var] U\<heavy_comma> X \<longmapsto> Z \<rbrace> \<t>\<h>\<r>\<o>\<w>\<s> E
+  \<open> \<p>\<r>\<o>\<c> g \<lbrace> R\<heavy_comma> y \<Ztypecolon> \<v>\<a>\<r>[var] U\<heavy_comma> \<blangle> X \<brangle> \<longmapsto> Z \<rbrace> \<t>\<h>\<r>\<o>\<w>\<s> E
 \<Longrightarrow> pred_option (\<lambda>TY'. TY = TY') (varname.type var) @action infer_var_type
 \<Longrightarrow> \<phi>SemType (y \<Ztypecolon> U) TY
-\<Longrightarrow> \<p>\<r>\<o>\<c> (op_set_var var TY raw \<ggreater> g) \<lbrace> R\<heavy_comma> (x \<Ztypecolon> Var var T \<heavy_comma> y \<Ztypecolon> \<v>\<a>\<l>[raw] U\<heavy_comma> X) \<longmapsto> Z \<rbrace> \<t>\<h>\<r>\<o>\<w>\<s> E \<close>
+\<Longrightarrow> \<p>\<r>\<o>\<c> (op_set_var var TY raw \<ggreater> g) \<lbrace> R\<heavy_comma> \<blangle> x \<Ztypecolon> Var var T \<heavy_comma> y \<Ztypecolon> \<v>\<a>\<l>[raw] U\<heavy_comma> X \<brangle> \<longmapsto> Z \<rbrace> \<t>\<h>\<r>\<o>\<w>\<s> E \<close>
   \<medium_left_bracket> premises G and P and [\<phi>reason]
     op_set_var P G
   \<medium_right_bracket> .. .
 
 lemma "__new_var_rule__":
   \<open> (\<And>var. varname.type var \<equiv> TY
-              \<Longrightarrow> \<p>\<r>\<o>\<c> g var \<lbrace> R\<heavy_comma> \<u>\<n>\<i>\<n>\<i>\<t>\<e>\<d> \<v>\<a>\<r>[var]\<heavy_comma> X \<longmapsto> \<lambda>ret. Z ret \<heavy_comma> () \<Ztypecolon> Var var \<phi>Any
+              \<Longrightarrow> \<p>\<r>\<o>\<c> g var \<lbrace> R\<heavy_comma> \<u>\<n>\<i>\<n>\<i>\<t>\<e>\<d> \<v>\<a>\<r>[var]\<heavy_comma> \<blangle> X \<brangle> \<longmapsto> \<lambda>ret. Z ret \<heavy_comma> () \<Ztypecolon> Var var \<phi>Any
                              \<rbrace> \<t>\<h>\<r>\<o>\<w>\<s> (\<lambda>e. E e\<heavy_comma> () \<Ztypecolon> Var var \<phi>Any))
-\<Longrightarrow> \<p>\<r>\<o>\<c> op_var_scope TYPE('a::VALs) TY g \<lbrace> R\<heavy_comma> X \<longmapsto> Z \<rbrace> \<t>\<h>\<r>\<o>\<w>\<s> E \<close>
+\<Longrightarrow> \<p>\<r>\<o>\<c> op_var_scope TYPE('a::VALs) TY g \<lbrace> R\<heavy_comma> \<blangle> X \<brangle> \<longmapsto> Z \<rbrace> \<t>\<h>\<r>\<o>\<w>\<s> E \<close>
   \<medium_left_bracket> premises G
     op_var_scope[where TY=\<open>TY\<close>] \<medium_left_bracket> premises [\<phi>reason for \<open>varname.type var \<equiv> _\<close>] G \<medium_right_bracket>.
   \<medium_right_bracket> .. .
@@ -402,11 +402,11 @@ lemma "__new_var_rule__":
 
 lemma "__set_new_var_rule__":
   \<open> (\<And>var. varname.type var \<equiv> Some TY
-              \<Longrightarrow> \<p>\<r>\<o>\<c> g var \<lbrace> R\<heavy_comma> y \<Ztypecolon> \<v>\<a>\<r>[var] U\<heavy_comma> X \<longmapsto> \<lambda>ret. Z ret \<heavy_comma> () \<Ztypecolon> Var var \<phi>Any
+              \<Longrightarrow> \<p>\<r>\<o>\<c> g var \<lbrace> R\<heavy_comma> y \<Ztypecolon> \<v>\<a>\<r>[var] U\<heavy_comma> \<blangle> X \<brangle> \<longmapsto> \<lambda>ret. Z ret \<heavy_comma> () \<Ztypecolon> Var var \<phi>Any
                              \<rbrace> \<t>\<h>\<r>\<o>\<w>\<s> (\<lambda>e. E e\<heavy_comma> () \<Ztypecolon> Var var \<phi>Any ))
 \<Longrightarrow> \<phi>SemType (y \<Ztypecolon> U) TY
 \<Longrightarrow> \<p>\<r>\<o>\<c> op_var_scope TYPE('a::VALs) (Some TY) (\<lambda>var. op_set_var var TY raw \<ggreater> g var)
-     \<lbrace> R\<heavy_comma> (y \<Ztypecolon> \<v>\<a>\<l>[raw] U\<heavy_comma> X) \<longmapsto> Z \<rbrace> \<t>\<h>\<r>\<o>\<w>\<s> E \<close>
+     \<lbrace> R\<heavy_comma> \<blangle> y \<Ztypecolon> \<v>\<a>\<l>[raw] U\<heavy_comma> X \<brangle> \<longmapsto> Z \<rbrace> \<t>\<h>\<r>\<o>\<w>\<s> E \<close>
   \<medium_left_bracket> premises G and [\<phi>reason]
     op_var_scope[where TY=\<open>Some TY\<close>] \<medium_left_bracket> premises [\<phi>reason for \<open>varname.type var \<equiv> _\<close>]
       op_set_var G
@@ -415,11 +415,11 @@ lemma "__set_new_var_rule__":
 
 lemma "__set_new_var_noty_rule__":
   \<open> (\<And>var. varname.type var \<equiv> None
-              \<Longrightarrow> \<p>\<r>\<o>\<c> g var \<lbrace> R\<heavy_comma> y \<Ztypecolon> \<v>\<a>\<r>[var] U\<heavy_comma> X \<longmapsto> \<lambda>ret. Z ret \<heavy_comma> () \<Ztypecolon> Var var \<phi>Any
+              \<Longrightarrow> \<p>\<r>\<o>\<c> g var \<lbrace> R\<heavy_comma> y \<Ztypecolon> \<v>\<a>\<r>[var] U\<heavy_comma> \<blangle> X \<brangle> \<longmapsto> \<lambda>ret. Z ret \<heavy_comma> () \<Ztypecolon> Var var \<phi>Any
                              \<rbrace> \<t>\<h>\<r>\<o>\<w>\<s> (\<lambda>e. E e\<heavy_comma> () \<Ztypecolon> Var var \<phi>Any))
 \<Longrightarrow> \<phi>SemType (y \<Ztypecolon> U) TY
 \<Longrightarrow> \<p>\<r>\<o>\<c> op_var_scope TYPE('a::VALs) None (\<lambda>var. op_set_var var TY raw \<ggreater> g var)
-     \<lbrace> R\<heavy_comma> (y \<Ztypecolon> \<v>\<a>\<l>[raw] U\<heavy_comma> X) \<longmapsto> Z \<rbrace> \<t>\<h>\<r>\<o>\<w>\<s> E \<close>
+     \<lbrace> R\<heavy_comma> \<blangle> y \<Ztypecolon> \<v>\<a>\<l>[raw] U\<heavy_comma> X \<brangle> \<longmapsto> Z \<rbrace> \<t>\<h>\<r>\<o>\<w>\<s> E \<close>
   \<medium_left_bracket> premises G and [\<phi>reason]
     op_var_scope[where TY=None] \<medium_left_bracket> premises [\<phi>reason for \<open>varname.type var \<equiv> _\<close>]
       op_set_var G
